src/Zulib/verify.sh
@@ -1,6 +1,6 @@
 #!/bin/sh
 
-mono ../../packages/ZFStar/tools/fstar.exe \
+mono ../../../FStar/bin/fstar.exe \
      --smt ../../packages/zen_z3_linux/output/z3-linux \
      --prims fstar/prims.fst \
      --no_default_includes \
